Fixed aux proofs

execution/theories/BlockchainSolanav2.v
@@ -92,68 +92,65 @@ Record AccountInformation :=
 
 MetaCoq Run (make_setters AccountInformation).
 
+Print Bool.reflect.
+
 Class AccountGetters :=
   build_account_getters {
     get_account_address : AccountInformation -> Address;       (* Account address *)
+    get_account_address_spec : forall (acc : AccountInformation),
+            get_account_address acc = account_address acc;
     get_account_is_writable : AccountInformation -> bool;      (* Can the account be written to *)
+    get_account_is_writable_spec : forall (acc : AccountInformation),
+            get_account_is_writable acc = account_is_writable acc;
     get_account_is_signer : AccountInformation -> bool;        (* Has the account signed the transaction *)
+    get_account_is_signer_spec : forall (acc : AccountInformation),
+            get_account_is_signer acc = account_is_signer acc;
     get_account_balance : AccountInformation -> Amount;        (* Account balance *)
+    get_account_balance_spec : forall (acc : AccountInformation),
+            get_account_balance acc = account_balance acc;
     get_account_state : AccountInformation -> SerializedValue; (* Account data *)
+    get_account_state_spec : forall (acc : AccountInformation),
+            get_account_state acc = account_state acc;
     get_account_owner_address : AccountInformation -> Address; (* Account owner address *)
+    get_account_owner_address_spec : forall (acc : AccountInformation),
+            get_account_owner_address acc = account_owner_address acc;
     get_account_is_executable : AccountInformation -> bool;    (* Is the account a program *)
+    get_account_is_executable_spec : forall (acc : AccountInformation),
+            get_account_is_executable acc = account_is_executable acc;
   }.
 
 Global Opaque get_account_address get_account_state get_account_balance get_account_owner_address
               get_account_is_signer get_account_is_writable get_account_is_executable.
 
-Lemma get_account_address_correct `{AccountGetters} acc addr1 addr2 : 
-  account_address acc = addr1 ->
-  get_account_address acc = addr2 -> 
-  addr1 = addr2 ->
+Lemma get_account_address_correct `{AccountGetters} acc : 
   account_address acc = get_account_address acc.
-Proof. easy. Qed.
+Proof. destruct (get_account_address_spec acc); auto. Qed.
 
-Lemma get_account_state_correct `{AccountGetters} acc st1 st2 : 
-  account_state acc = st1 ->
-  get_account_state acc = st2 ->
-  st1 = st2 ->
+Lemma get_account_state_correct `{AccountGetters} acc : 
   account_state acc = get_account_state acc.
-Proof. easy. Qed.
+Proof. destruct (get_account_state_spec acc); auto. Qed.
 
-Lemma get_account_balance_correct `{AccountGetters} acc bal1 bal2 : 
-  account_balance acc = bal1 ->
-  get_account_balance acc = bal2 -> 
-  bal1 = bal2 ->
+Lemma get_account_balance_correct `{AccountGetters} acc : 
   account_balance acc = get_account_balance acc.
-Proof. easy. Qed.
+Proof. destruct (get_account_balance_spec acc); auto. Qed.
 
-Lemma get_account_owner_address_correct `{AccountGetters} acc owner_addr1 owner_addr2 : 
-  account_owner_address acc = owner_addr1 ->
-  get_account_owner_address acc = owner_addr2 ->
-  owner_addr1 = owner_addr2 -> 
+Lemma get_account_owner_address_correct `{AccountGetters} acc : 
   account_owner_address acc = get_account_owner_address acc.
-Proof. easy. Qed.
+Proof.
+  destruct (get_account_owner_address_spec acc); auto.
+ Qed. 
 
-Lemma get_account_is_signer_correct `{AccountGetters} acc x1 x2 : 
-  account_is_signer acc = x1 ->
-  get_account_is_signer acc = x2 ->
-  x1 = x2 -> 
+Lemma get_account_is_signer_correct `{AccountGetters} acc : 
   account_is_signer acc = get_account_is_signer acc.
-Proof. easy. Qed.
+Proof. destruct (get_account_is_signer_spec acc); auto. Qed.
 
-Lemma get_account_is_writable_correct `{AccountGetters} acc x1 x2 : 
-  account_is_writable acc = x1 ->
-  get_account_is_writable acc = x2 ->
-  x1 = x2 -> 
+Lemma get_account_is_writable_correct `{AccountGetters} acc : 
   account_is_writable acc = get_account_is_writable acc.
-Proof. easy. Qed.
+Proof. destruct (get_account_is_writable_spec acc); auto. Qed.
 
-Lemma get_account_is_executable_correct `{AccountGetters} acc x1 x2 : 
-  account_is_executable acc = x1 ->
-  get_account_is_executable acc = x2 -> 
-  x1 = x2 ->
+Lemma get_account_is_executable_correct `{AccountGetters} acc :
   account_is_executable acc = get_account_is_executable acc.
-Proof. easy. Qed.
+Proof. destruct (get_account_is_executable_spec acc); auto. Qed.
 
 Definition SliceAccountInformation := list AccountInformation.
 Global Opaque SliceAccountInformation.
